\documentclass{review-sheet}
\homework{9}

\begin{document}
\begin{problem}{\S 1}
  Let $S,T:\R^2\to \R^3$ be the linear maps determined by
  \begin{align*}
    S(1,1)=(2,-1,3), && S(1,-1) = (2,-2,4)\\
    T(1,0)=(4,0,0), && T(0,1) = (-4,-1,0)
  .\end{align*}
  Compute:
  \begin{enumerate}[label=(\alph*)]
    \item $(-S)(4,0)$
    \item  $(-S+T)(4,0)$
    \item  $(-S+T)(4,0)+(-S+T)(-1,3)+(-S+T)(-2,-2)+(-S+T)(-1,-1)$ 
    \item $ \mc{M}(-S)$
    \item $\mc{M}(T)$
    \item $-\mc{M}(S)+\mc{M}(T)$
  \end{enumerate}
\end{problem}

\begin{solution}
  We first find the matrices of $S$ and $T$ with respect to the standard basis:
  \begin{align*}
    \mc{M}(S)=\begin{pmatrix} 2&0\\-\frac{3}{2}&\frac{1}{2}\\\frac{7}{2}&-\frac{1}{2}
      \end{pmatrix},&& \mc{M}(T)=\begin{pmatrix} 4&-4\\0&-1\\0&0 \end{pmatrix} 
  .\end{align*}

  \begin{enumerate}[label=(\alph*)]
    \item $-S(4,0)=(-8,6,-14)$.
    \item  $(-S+T)(4,0)=(8,6,-14)$.
    \item  $(-S+T)(4,0)+(-S+T)(1,3)+(-S+T)(-2,-2)+(-S+T)(-1,-1)=(0,0,0)$.
    \item $\mc{M}(-S)=\begin{pmatrix} -2&0\\\frac{3}{2}&-\frac{1}{2}\\-\frac{7}{2}&\frac{1}{2} \end{pmatrix} $ 
    \item $\mc{M}(T)=\begin{pmatrix} 4&-4\\0&-1\\0&0 \end{pmatrix}$
    \item $-\mc{M}(S)+\mc{M}(T)=\begin{pmatrix}
      2&-4\\\frac{3}{2}&-\frac{3}{2}\\-\frac{7}{2}&\frac{1}{2} \end{pmatrix} $
  \end{enumerate}
\end{solution}

\begin{problem}{\S 2}
  Write the linear map \[
    T:\mc{P}_3(\R)\to \mc{P}_3(\R)
  \] given by \[
    T(f) = f+f'+f''
  \] as a matrix with respect to the basis \[
    1,\ x-2,\ (x-2)^2,\ (x-2)^3
  \] for both the domain and codomain.
\end{problem}

\begin{solution}
  We have
  \begin{align*}
    T(1)&=1+0+0=1\\
    T(x-2)&=x-2+1+0=x-1\\
    T((x-2)^2)&= (x-2)^2+2(x-2)+2=x^2-2x+2 \\
    T((x-2)^3)&= (x-2)^3+2(x-2)^2+4(x-2)=x^3-3x^2+6x-8
  .\end{align*}
  So,
  \begin{align*}
    T(1) &= (1,0,0,0)\\
    T(x-2)&= x-1=(x-2)+1=(1,1,0,0) \\
    T((x-2)^2)&= x^2-2x+2=(x-2)^2+2x-2=(x-2)^2+2(x-2)+2=(2,2,1,0) \\
    T((x-2)^3)&= x^3-3x^2+6x-8=(x-2)^3+3x^2-6x=(x-2)^3+3(x-2)^2+6(x-2)=(0,6,3,1)
  \end{align*}
  and so \[
    \mc{M}(T)=\begin{pmatrix} 1&1&2&0\\0&1&2&6\\0&0&1&3\\0&0&0&1 \end{pmatrix} 
  \] with respect to the basis $1,x-2,(x-2)^2,(x-2)^3$.
\end{solution}







\end{document}
